add modq and rm montgomery from qinv

code/k256/Hacl.Impl.K256.Qinv.fst
@@ -16,44 +16,23 @@ module S = Spec.K256
 module SI = Hacl.Spec.K256.Qinv
 
 module BE = Hacl.Impl.Exponentiation
-module BN = Hacl.Bignum
-module BM = Hacl.Bignum.Montgomery
-
 module SD = Hacl.Spec.Bignum.Definitions
-module SM = Hacl.Spec.Bignum.Montgomery
-module M = Hacl.Spec.Montgomery.Lemmas
 
 #set-options "--z3rlimit 50 --fuel 0 --ifuel 0"
 
-(** Montgomery arithmetic for modular exponentiation and field inversion *)
+unfold
+let linv_ctx (a:LSeq.lseq uint64 0) : Type0 = True
 
-inline_for_extraction noextract
-let km = BM.mk_runtime_mont #U64 qnlimb
-
-inline_for_extraction noextract
-let linv_ctx (a:LSeq.lseq uint64 4) : Type0 =
-  SD.bn_v #U64 #4 a == S.q
-
-inline_for_extraction noextract
+unfold
 let linv (a:LSeq.lseq uint64 4) : Type0 =
   SD.bn_v #U64 #4 a < S.q
 
-inline_for_extraction noextract
-let refl (aM:LSeq.lseq uint64 4{linv aM}) : GTot S.qelem =
-  let mu = make_mu0 () in
-  M.from_mont_lemma 64 4 S.q (v mu) (SD.bn_v aM);
-  M.from_mont 64 4 S.q (v mu) (SD.bn_v aM)
-
+unfold
+let refl (a:LSeq.lseq uint64 4{linv a}) : GTot S.qelem =
+  SD.bn_v #U64 #4 a
 
 inline_for_extraction noextract
-let linv_ctxs (h:mem) (n:qelem) = linv_ctx (as_seq h n)
-inline_for_extraction noextract
-let linvs (h:mem) (aM:qelem) = linv (as_seq h aM)
-inline_for_extraction noextract
-let refls (h:mem) (aM:qelem{linvs h aM}) = refl (as_seq h aM)
-
-inline_for_extraction noextract
-let mk_to_k256_scalar_concrete_ops : BE.to_concrete_ops U64 4ul 4ul = {
+let mk_to_k256_scalar_concrete_ops : BE.to_concrete_ops U64 4ul 0ul = {
   BE.t_spec = S.qelem;
   BE.concr_ops = SI.mk_nat_mod_concrete_ops;
   BE.linv_ctx = linv_ctx;
@@ -62,105 +41,52 @@ let mk_to_k256_scalar_concrete_ops : BE.to_concrete_ops U64 4ul 4ul = {
 }
 
 
-val qmul_mont : BE.lmul_st U64 4ul 4ul mk_to_k256_scalar_concrete_ops
-[@CInline]
-let qmul_mont n aM bM resM =
-  let h0 = ST.get () in
-  [@inline_let]
-  let mu = make_mu0 () in
-  SM.bn_mont_mul_lemma (as_seq h0 n) mu (as_seq h0 aM) (as_seq h0 bM);
-  M.from_mont_mul_lemma 64 4 (qas_nat h0 n) (v mu) (qas_nat h0 aM) (qas_nat h0 bM);
-  km.BM.mul n mu aM bM resM
-
-
-val qsqr_mont : BE.lsqr_st U64 4ul 4ul mk_to_k256_scalar_concrete_ops
-[@CInline]
-let qsqr_mont n aM resM =
-  let h0 = ST.get () in
-  [@inline_let]
-  let mu = make_mu0 () in
-  SM.bn_mont_sqr_lemma (as_seq h0 n) mu (as_seq h0 aM);
-  M.from_mont_mul_lemma 64 4 (qas_nat h0 n) (v mu) (qas_nat h0 aM) (qas_nat h0 aM);
-  km.BM.sqr n mu aM resM
+inline_for_extraction noextract
+val mul_mod : BE.lmul_st U64 4ul 0ul mk_to_k256_scalar_concrete_ops
+let mul_mod ctx x y xy = qmul xy x y
 
 
 inline_for_extraction noextract
-let mk_k256_scalar_concrete_ops : BE.concrete_ops U64 4ul 4ul = {
+val sqr_mod : BE.lsqr_st U64 4ul 0ul mk_to_k256_scalar_concrete_ops
+let sqr_mod ctx x xx = qsqr xx x
+
+
+inline_for_extraction noextract
+let mk_k256_scalar_concrete_ops : BE.concrete_ops U64 4ul 0ul = {
   BE.to = mk_to_k256_scalar_concrete_ops;
-  BE.lmul = qmul_mont;
-  BE.lsqr = qsqr_mont;
+  BE.lmul = mul_mod;
+  BE.lsqr = sqr_mod;
 }
 
 
-val to_mont (n a aM:qelem) : Stack unit
+val qsquare_times_in_place (out:qelem) (b:size_t) : Stack unit
   (requires fun h ->
-    live h n /\ live h a /\ live h aM /\
-    disjoint n a /\ disjoint n aM /\ disjoint a aM /\
-    linvs h a /\ linv_ctxs h n)
-  (ensures  fun h0 _ h1 -> modifies (loc aM) h0 h1 /\
-    linvs h1 aM /\ refls h1 aM == qas_nat h0 a)
-[@CInline]
-let to_mont n a aM =
-  push_frame ();
-  let r2 = create qnlimb (u64 0) in
-  make_u64_4 r2 (make_r2_modq ());
-  let h0 = ST.get () in
-  [@inline_let]
-  let mu = make_mu0 () in
-  km.BM.to n mu r2 a aM;
-  SM.bn_to_mont_lemma (as_seq h0 n) mu (as_seq h0 r2) (as_seq h0 a);
-  M.from_to_mont_lemma 64 4 (qas_nat h0 n) (v mu) (qas_nat h0 a);
-  pop_frame ()
-
-
-val from_mont (n aM a:qelem) : Stack unit
-  (requires fun h ->
-    live h n /\ live h a /\ live h aM /\
-    disjoint n a /\ disjoint n aM /\ disjoint a aM /\
-    linvs h aM /\ linv_ctxs h n)
-  (ensures  fun h0 _ h1 -> modifies (loc a) h0 h1 /\
-    linvs h1 a /\ qas_nat h1 a == refls h0 aM)
-[@CInline]
-let from_mont n aM a =
-  let h0 = ST.get () in
-  [@inline_let]
-  let mu = make_mu0 () in
-  km.BM.from n mu aM a;
-  SM.bn_from_mont_lemma (as_seq h0 n) mu (as_seq h0 aM)
-
-
-val qsquare_times_in_place (n out:qelem) (b:size_t) : Stack unit
-  (requires fun h ->
-    live h n /\ live h out /\ disjoint n out /\
-    linvs h out /\ linv_ctxs h n)
-  (ensures  fun h0 _ h1 -> modifies (loc out) h0 h1 /\ linvs h1 out /\
-    refls h1 out == SI.qsquare_times (refls h0 out) (v b))
+    live h out /\ qe_lt_q h out)
+  (ensures  fun h0 _ h1 -> modifies (loc out) h0 h1 /\ qe_lt_q h1 out /\
+    qas_nat h1 out == SI.qsquare_times (qas_nat h0 out) (v b))
 
 [@CInline]
-let qsquare_times_in_place n out b =
-  BE.lexp_pow_in_place 4ul 4ul mk_k256_scalar_concrete_ops n out b
+let qsquare_times_in_place out b =
+  BE.lexp_pow_in_place 4ul 0ul mk_k256_scalar_concrete_ops (null uint64) out b
 
 
-val qsquare_times (n out a:qelem) (b:size_t) : Stack unit
+val qsquare_times (out a:qelem) (b:size_t) : Stack unit
   (requires fun h ->
-    live h out /\ live h a /\ live h n /\
-    disjoint out a /\ disjoint out n /\ disjoint a n /\
-    linvs h a /\ linv_ctxs h n)
-  (ensures  fun h0 _ h1 -> modifies (loc out) h0 h1 /\ linvs h1 out /\
-    refls h1 out == SI.qsquare_times (refls h0 a) (v b))
+    live h out /\ live h a /\ disjoint out a /\
+    qe_lt_q h a)
+  (ensures  fun h0 _ h1 -> modifies (loc out) h0 h1 /\ qe_lt_q h1 a /\
+    qas_nat h1 out == SI.qsquare_times (qas_nat h0 a) (v b))
 
 [@CInline]
-let qsquare_times n out a b =
-  BE.lexp_pow2 4ul 4ul mk_k256_scalar_concrete_ops n a b out
+let qsquare_times out a b =
+  BE.lexp_pow2 4ul 0ul mk_k256_scalar_concrete_ops (null uint64) a b out
 
 
 inline_for_extraction noextract
-val qinv1 (n f x_10 x_11 x_101 x_111 x_1001 x_1011 x_1101:qelem) : Stack unit
+val qinv1 (f x_10 x_11 x_101 x_111 x_1001 x_1011 x_1101:qelem) : Stack unit
   (requires fun h ->
-    live h n /\ live h f /\ live h x_10 /\ live h x_11 /\ live h x_101 /\
+    live h f /\ live h x_10 /\ live h x_11 /\ live h x_101 /\
     live h x_111 /\ live h x_1001 /\ live h x_1011 /\ live h x_1101 /\
-    disjoint n f /\ disjoint n x_10 /\ disjoint n x_11 /\ disjoint n x_101 /\
-    disjoint n x_111 /\ disjoint n x_1001 /\ disjoint n x_1011 /\ disjoint n x_1101 /\
     disjoint f x_10 /\ disjoint f x_11 /\ disjoint f x_101 /\
     disjoint f x_111 /\ disjoint f x_1001 /\ disjoint f x_1011 /\
     disjoint f x_1101 /\ disjoint x_10 x_11 /\ disjoint x_10 x_101 /\
@@ -170,380 +96,375 @@ val qinv1 (n f x_10 x_11 x_101 x_111 x_1001 x_1011 x_1101:qelem) : Stack unit
     disjoint x_101 x_111 /\ disjoint x_101 x_1001 /\ disjoint x_101 x_1011 /\
     disjoint x_101 x_1101 /\ disjoint x_111 x_1001 /\ disjoint x_111 x_1011 /\
     disjoint x_111 x_1101 /\ disjoint x_1001 x_1011 /\ disjoint x_1001 x_1101 /\
-    disjoint x_1011 x_1101 /\ linvs h f /\ linv_ctxs h n)
+    disjoint x_1011 x_1101 /\ qe_lt_q h f)
   (ensures  fun h0 _ h1 ->
     modifies (loc x_10 |+| loc x_11 |+| loc x_101 |+|
       loc x_111 |+| loc x_1001 |+| loc x_1011 |+| loc x_1101) h0 h1 /\
-   (let _x_10 = SI.qsquare_times (refls h0 f) 1 in
-    let _x_11 = S.qmul _x_10 (refls h0 f) in
+   (let _x_10 = SI.qsquare_times (qas_nat h0 f) 1 in
+    let _x_11 = S.qmul _x_10 (qas_nat h0 f) in
     let _x_101 = S.qmul _x_10 _x_11 in
     let _x_111 = S.qmul _x_10 _x_101 in
     let _x_1001 = S.qmul _x_10 _x_111 in
     let _x_1011 = S.qmul _x_10 _x_1001 in
     let _x_1101 = S.qmul _x_10 _x_1011 in
-    linvs h1 x_10 /\ refls h1 x_10 == _x_10 /\
-    linvs h1 x_11 /\ refls h1 x_11 == _x_11 /\
-    linvs h1 x_101 /\ refls h1 x_101 == _x_101 /\
-    linvs h1 x_111 /\ refls h1 x_111 == _x_111 /\
-    linvs h1 x_1001 /\ refls h1 x_1001 == _x_1001 /\
-    linvs h1 x_1011 /\ refls h1 x_1011 == _x_1011 /\
-    linvs h1 x_1101 /\ refls h1 x_1101 == _x_1101))
+    qas_nat h1 x_10 == _x_10 /\ qe_lt_q h1 x_10 /\
+    qas_nat h1 x_11 == _x_11 /\ qe_lt_q h1 x_11 /\
+    qas_nat h1 x_101 == _x_101 /\ qe_lt_q h1 x_101 /\
+    qas_nat h1 x_111 == _x_111 /\ qe_lt_q h1 x_111 /\
+    qas_nat h1 x_1001 == _x_1001 /\ qe_lt_q h1 x_1001 /\
+    qas_nat h1 x_1011 == _x_1011 /\ qe_lt_q h1 x_1011 /\
+    qas_nat h1 x_1101 == _x_1101 /\ qe_lt_q h1 x_1101))
 
-let qinv1 n f x_10 x_11 x_101 x_111 x_1001 x_1011 x_1101 =
+let qinv1 f x_10 x_11 x_101 x_111 x_1001 x_1011 x_1101 =
   let h0 = ST.get () in
-  qsquare_times n x_10 f 1ul;
+  qsquare_times x_10 f 1ul;
   let h1 = ST.get () in
-  assert (refls h1 x_10 == SI.qsquare_times (refls h0 f) 1);
+  assert (qas_nat h1 x_10 == SI.qsquare_times (qas_nat h0 f) 1);
 
-  qmul_mont n x_10 f x_11;
+  qmul x_11 x_10 f;
   let h2 = ST.get () in
-  assert (refls h2 x_11 == S.qmul (refls h1 x_10) (refls h0 f));
+  assert (qas_nat h2 x_11 == S.qmul (qas_nat h1 x_10) (qas_nat h0 f));
 
-  qmul_mont n x_10 x_11 x_101;
+  qmul x_101 x_10 x_11;
   let h3 = ST.get () in
-  assert (refls h3 x_101 == S.qmul (refls h1 x_10) (refls h2 x_11));
+  assert (qas_nat h3 x_101 == S.qmul (qas_nat h1 x_10) (qas_nat h2 x_11));
 
-  qmul_mont n x_10 x_101 x_111;
+  qmul x_111 x_10 x_101;
   let h4 = ST.get () in
-  assert (refls h4 x_111 == S.qmul (refls h1 x_10) (refls h3 x_101));
+  assert (qas_nat h4 x_111 == S.qmul (qas_nat h1 x_10) (qas_nat h3 x_101));
 
-  qmul_mont n x_10 x_111 x_1001;
+  qmul x_1001 x_10 x_111;
   let h5 = ST.get () in
-  assert (refls h5 x_1001 == S.qmul (refls h1 x_10) (refls h4 x_111));
+  assert (qas_nat h5 x_1001 == S.qmul (qas_nat h1 x_10) (qas_nat h4 x_111));
 
-  qmul_mont n x_10 x_1001 x_1011;
+  qmul x_1011 x_10 x_1001;
   let h6 = ST.get () in
-  assert (refls h6 x_1011 == S.qmul (refls h1 x_10) (refls h5 x_1001));
+  assert (qas_nat h6 x_1011 == S.qmul (qas_nat h1 x_10) (qas_nat h5 x_1001));
 
-  qmul_mont n x_10 x_1011 x_1101;
+  qmul x_1101 x_10 x_1011;
   let h7 = ST.get () in
-  assert (refls h7 x_1101 == S.qmul (refls h1 x_10) (refls h6 x_1011))
+  assert (qas_nat h7 x_1101 == S.qmul (qas_nat h1 x_10) (qas_nat h6 x_1011))
 
 
 inline_for_extraction noextract
-val qinv2 (n x_11 x_1011 x_1101 x6 x8 x14: qelem) : Stack unit
+val qinv2 (x_11 x_1011 x_1101 x6 x8 x14: qelem) : Stack unit
   (requires fun h ->
-    live h n /\ live h x_11 /\ live h x_1011 /\
-    live h x_1101 /\ live h x6 /\ live h x8 /\ live h x14 /\
-    disjoint n x_11 /\ disjoint n x_1011 /\ disjoint n x_1101 /\
-    disjoint n x6 /\ disjoint n x8 /\ disjoint n x14 /\
+    live h x_11 /\ live h x_1011 /\ live h x_1101 /\
+    live h x6 /\ live h x8 /\ live h x14 /\
     disjoint x_11 x6 /\ disjoint x_11 x8 /\ disjoint x_11 x14 /\
     disjoint x_1011 x6 /\ disjoint x_1011 x8 /\ disjoint x_1011 x14 /\
     disjoint x_1101 x6 /\ disjoint x_1101 x8 /\ disjoint x_1101 x14 /\
     disjoint x6 x8 /\ disjoint x6 x14 /\ disjoint x8 x14 /\
-    linvs h x_11 /\ linvs h x_1011 /\ linvs h x_1101 /\ linv_ctxs h n)
+    qe_lt_q h x_11 /\ qe_lt_q h x_1011 /\ qe_lt_q h x_1101)
   (ensures fun h0 _ h1 -> modifies (loc x6 |+| loc x8 |+| loc x14) h0 h1 /\
-   (let _x6 = S.qmul (SI.qsquare_times (refls h0 x_1101) 2) (refls h0 x_1011) in
-    let _x8 = S.qmul (SI.qsquare_times _x6 2) (refls h0 x_11) in
+   (let _x6 = S.qmul (SI.qsquare_times (qas_nat h0 x_1101) 2) (qas_nat h0 x_1011) in
+    let _x8 = S.qmul (SI.qsquare_times _x6 2) (qas_nat h0 x_11) in
     let _x14 = S.qmul (SI.qsquare_times _x8 6) _x6 in
-    linvs h1 x6 /\ refls h1 x6 == _x6 /\
-    linvs h1 x8 /\ refls h1 x8 == _x8 /\
-    linvs h1 x14 /\ refls h1 x14 == _x14))
+    qas_nat h1 x6 == _x6 /\ qe_lt_q h1 x6 /\
+    qas_nat h1 x8 == _x8 /\ qe_lt_q h1 x8 /\
+    qas_nat h1 x14 == _x14 /\ qe_lt_q h1 x14))
 
-let qinv2 n x_11 x_1011 x_1101 x6 x8 x14 =
+let qinv2 x_11 x_1011 x_1101 x6 x8 x14 =
   let h0 = ST.get () in
-  qsquare_times n x6 x_1101 2ul;
-  qmul_mont n x6 x_1011 x6;
+  qsquare_times x6 x_1101 2ul;
+  qmul x6 x6 x_1011;
   let h1 = ST.get () in
-  assert (refls h1 x6 == S.qmul (SI.qsquare_times (refls h0 x_1101) 2) (refls h0 x_1011));
+  assert (qas_nat h1 x6 == S.qmul (SI.qsquare_times (qas_nat h0 x_1101) 2) (qas_nat h0 x_1011));
 
-  qsquare_times n x8 x6 2ul;
-  qmul_mont n x8 x_11 x8;
+  qsquare_times x8 x6 2ul;
+  qmul x8 x8 x_11;
   let h2 = ST.get () in
-  assert (refls h2 x8 == S.qmul (SI.qsquare_times (refls h1 x6) 2) (refls h0 x_11));
+  assert (qas_nat h2 x8 == S.qmul (SI.qsquare_times (qas_nat h1 x6) 2) (qas_nat h0 x_11));
 
-  qsquare_times n x14 x8 6ul;
-  qmul_mont n x14 x6 x14;
+  qsquare_times x14 x8 6ul;
+  qmul x14 x14 x6;
   let h3 = ST.get () in
-  assert (refls h3 x14 == S.qmul (SI.qsquare_times (refls h2 x8) 6) (refls h1 x6))
+  assert (qas_nat h3 x14 == S.qmul (SI.qsquare_times (qas_nat h2 x8) 6) (qas_nat h1 x6))
 
 
 inline_for_extraction noextract
-val qinv3 (n tmp x14: qelem) : Stack unit
+val qinv3 (tmp x14: qelem) : Stack unit
   (requires fun h ->
-    live h n /\ live h tmp /\ live h x14 /\
-    disjoint n tmp /\ disjoint n x14 /\ disjoint tmp x14 /\
-    linvs h x14 /\ linv_ctxs h n)
+    live h tmp /\ live h x14 /\ disjoint tmp x14 /\
+    qe_lt_q h x14)
   (ensures  fun h0 _ h1 -> modifies (loc tmp) h0 h1 /\
-    linvs h1 tmp /\ refls h1 tmp == SI.qinv_r0_r1 (refls h0 x14))
+    qas_nat h1 tmp == SI.qinv_r0_r1 (qas_nat h0 x14) /\
+    qe_lt_q h1 tmp)
 
-let qinv3 n tmp x14 =
+let qinv3 tmp x14 =
   push_frame ();
   let x56 = create_qelem () in
 
   let h0 = ST.get () in
-  qsquare_times n tmp x14 14ul;
-  qmul_mont n tmp x14 tmp; //tmp = x28
+  qsquare_times tmp x14 14ul;
+  qmul tmp tmp x14; //tmp = x28
   let h1 = ST.get () in
-  assert (refls h1 tmp == S.qmul (SI.qsquare_times (refls h0 x14) 14) (refls h0 x14));
+  assert (qas_nat h1 tmp == S.qmul (SI.qsquare_times (qas_nat h0 x14) 14) (qas_nat h0 x14));
 
-  qsquare_times n x56 tmp 28ul;
-  qmul_mont n x56 tmp x56;
+  qsquare_times x56 tmp 28ul;
+  qmul x56 x56 tmp;
   let h2 = ST.get () in
-  assert (refls h2 x56 == S.qmul (SI.qsquare_times (refls h1 tmp) 28) (refls h1 tmp));
+  assert (qas_nat h2 x56 == S.qmul (SI.qsquare_times (qas_nat h1 tmp) 28) (qas_nat h1 tmp));
 
-  qsquare_times n tmp x56 56ul; //tmp = r0
-  qmul_mont n tmp x56 tmp;
+  qsquare_times tmp x56 56ul; //tmp = r0
+  qmul tmp tmp x56;
   let h3 = ST.get () in
-  assert (refls h3 tmp == S.qmul (SI.qsquare_times (refls h2 x56) 56) (refls h2 x56));
+  assert (qas_nat h3 tmp == S.qmul (SI.qsquare_times (qas_nat h2 x56) 56) (qas_nat h2 x56));
 
-  qsquare_times_in_place n tmp 14ul; //tmp = r1
-  qmul_mont n tmp x14 tmp;
+  qsquare_times_in_place tmp 14ul; //tmp = r1
+  qmul tmp tmp x14;
   let h4 = ST.get () in
-  assert (refls h4 tmp == S.qmul (SI.qsquare_times (refls h3 tmp) 14) (refls h0 x14));
+  assert (qas_nat h4 tmp == S.qmul (SI.qsquare_times (qas_nat h3 tmp) 14) (qas_nat h0 x14));
   pop_frame ()
 
 
 //r2; .. ;r8
 inline_for_extraction noextract
-val qinv4 (n tmp x_101 x_111 x_1011: qelem) : Stack unit
+val qinv4 (tmp x_101 x_111 x_1011: qelem) : Stack unit
   (requires fun h ->
-    live h n /\ live h tmp /\ live h x_101 /\ live h x_111 /\ live h x_1011 /\
-    disjoint n tmp /\ disjoint n x_101 /\ disjoint n x_111 /\ disjoint n x_1011 /\
+    live h tmp /\ live h x_101 /\ live h x_111 /\ live h x_1011 /\
     disjoint tmp x_101 /\ disjoint tmp x_111 /\ disjoint tmp x_1011 /\
-    linvs h tmp /\ linvs h x_101 /\ linvs h x_111 /\
-    linvs h x_1011 /\ linv_ctxs h n)
+    qe_lt_q h tmp /\ qe_lt_q h x_101 /\ qe_lt_q h x_111 /\ qe_lt_q h x_1011)
   (ensures  fun h0 _ h1 -> modifies (loc tmp) h0 h1 /\
-    linvs h1 tmp /\ refls h1 tmp == SI.qinv_r2_r8 (refls h0 tmp)
-      (refls h0 x_101) (refls h0 x_111) (refls h0 x_1011))
+    qas_nat h1 tmp == SI.qinv_r2_r8 (qas_nat h0 tmp)
+      (qas_nat h0 x_101) (qas_nat h0 x_111) (qas_nat h0 x_1011) /\
+    qe_lt_q h1 tmp)
 
-let qinv4 n tmp x_101 x_111 x_1011 =
+let qinv4 tmp x_101 x_111 x_1011 =
   let h0 = ST.get () in
-  qsquare_times_in_place n tmp 3ul;
-  qmul_mont n tmp x_101 tmp; //tmp = r2
+  qsquare_times_in_place tmp 3ul;
+  qmul tmp tmp x_101; //tmp = r2
   let h1 = ST.get () in
-  assert (refls h1 tmp == S.qmul (SI.qsquare_times (refls h0 tmp) 3) (refls h0 x_101));
+  assert (qas_nat h1 tmp == S.qmul (SI.qsquare_times (qas_nat h0 tmp) 3) (qas_nat h0 x_101));
 
-  qsquare_times_in_place n tmp 4ul;
-  qmul_mont n tmp x_111 tmp; //tmp = r3
+  qsquare_times_in_place tmp 4ul;
+  qmul tmp tmp x_111; //tmp = r3
   let h2 = ST.get () in
-  assert (refls h2 tmp == S.qmul (SI.qsquare_times (refls h1 tmp) 4) (refls h0 x_111));
+  assert (qas_nat h2 tmp == S.qmul (SI.qsquare_times (qas_nat h1 tmp) 4) (qas_nat h0 x_111));
 
-  qsquare_times_in_place n tmp 4ul;
-  qmul_mont n tmp x_101 tmp; //tmp = r4
+  qsquare_times_in_place tmp 4ul;
+  qmul tmp tmp x_101; //tmp = r4
   let h3 = ST.get () in
-  assert (refls h3 tmp == S.qmul (SI.qsquare_times (refls h2 tmp) 4) (refls h0 x_101));
+  assert (qas_nat h3 tmp == S.qmul (SI.qsquare_times (qas_nat h2 tmp) 4) (qas_nat h0 x_101));
 
-  qsquare_times_in_place n tmp 5ul;
-  qmul_mont n tmp x_1011 tmp; //tmp = r5
+  qsquare_times_in_place tmp 5ul;
+  qmul tmp tmp x_1011; //tmp = r5
   let h4 = ST.get () in
-  assert (refls h4 tmp == S.qmul (SI.qsquare_times (refls h3 tmp) 5) (refls h0 x_1011));
+  assert (qas_nat h4 tmp == S.qmul (SI.qsquare_times (qas_nat h3 tmp) 5) (qas_nat h0 x_1011));
 
-  qsquare_times_in_place n tmp 4ul;
-  qmul_mont n tmp x_1011 tmp; //tmp = r6
+  qsquare_times_in_place tmp 4ul;
+  qmul tmp tmp x_1011; //tmp = r6
   let h5 = ST.get () in
-  assert (refls h5 tmp == S.qmul (SI.qsquare_times (refls h4 tmp) 4) (refls h0 x_1011));
+  assert (qas_nat h5 tmp == S.qmul (SI.qsquare_times (qas_nat h4 tmp) 4) (qas_nat h0 x_1011));
 
-  qsquare_times_in_place n tmp 4ul;
-  qmul_mont n tmp x_111 tmp; //tmp = r7
+  qsquare_times_in_place tmp 4ul;
+  qmul tmp tmp x_111; //tmp = r7
   let h6 = ST.get () in
-  assert (refls h6 tmp == S.qmul (SI.qsquare_times (refls h5 tmp) 4) (refls h0 x_111));
+  assert (qas_nat h6 tmp == S.qmul (SI.qsquare_times (qas_nat h5 tmp) 4) (qas_nat h0 x_111));
 
-  qsquare_times_in_place n tmp 5ul;
-  qmul_mont n tmp x_111 tmp; //tmp = r8
+  qsquare_times_in_place tmp 5ul;
+  qmul tmp tmp x_111; //tmp = r8
   let h7 = ST.get () in
-  assert (refls h7 tmp == S.qmul (SI.qsquare_times (refls h6 tmp) 5) (refls h0 x_111))
+  assert (qas_nat h7 tmp == S.qmul (SI.qsquare_times (qas_nat h6 tmp) 5) (qas_nat h0 x_111))
 
 
 // r9; ..; r15
 inline_for_extraction noextract
-val qinv5 (n tmp x_101 x_111 x_1001 x_1101: qelem) : Stack unit
+val qinv5 (tmp x_101 x_111 x_1001 x_1101: qelem) : Stack unit
   (requires fun h ->
-    live h n /\ live h tmp /\ live h x_101 /\ live h x_111 /\
-    live h x_1001 /\ live h x_1101 /\ disjoint n tmp /\
-    disjoint n x_101 /\ disjoint n x_111 /\ disjoint n x_1001 /\
-    disjoint n x_1101 /\ disjoint tmp x_101 /\ disjoint tmp x_111 /\
-    disjoint tmp x_1001 /\ disjoint tmp x_1101 /\
-    linvs h tmp /\ linvs h x_101 /\ linvs h x_111 /\
-    linvs h x_1001 /\ linvs h x_1101 /\ linv_ctxs h n)
+    live h tmp /\ live h x_101 /\ live h x_111 /\
+    live h x_1001 /\ live h x_1101 /\ disjoint tmp x_101 /\
+    disjoint tmp x_111 /\ disjoint tmp x_1001 /\ disjoint tmp x_1101 /\
+    qe_lt_q h tmp /\ qe_lt_q h x_101 /\ qe_lt_q h x_111 /\
+    qe_lt_q h x_1001 /\ qe_lt_q h x_1101)
   (ensures  fun h0 _ h1 -> modifies (loc tmp) h0 h1 /\
-    linvs h1 tmp /\ refls h1 tmp == SI.qinv_r9_r15 (refls h0 tmp)
-      (refls h0 x_101) (refls h0 x_111) (refls h0 x_1001) (refls h0 x_1101))
+    qas_nat h1 tmp == SI.qinv_r9_r15 (qas_nat h0 tmp)
+      (qas_nat h0 x_101) (qas_nat h0 x_111) (qas_nat h0 x_1001) (qas_nat h0 x_1101) /\
+    qe_lt_q h1 tmp)
 
-let qinv5 n tmp x_101 x_111 x_1001 x_1101 =
+let qinv5 tmp x_101 x_111 x_1001 x_1101 =
   let h0 = ST.get () in
-  qsquare_times_in_place n tmp 6ul;
-  qmul_mont n tmp x_1101 tmp; //tmp = r9
+  qsquare_times_in_place tmp 6ul;
+  qmul tmp tmp x_1101; //tmp = r9
   let h1 = ST.get () in
-  assert (refls h1 tmp == S.qmul (SI.qsquare_times (refls h0 tmp) 6) (refls h0 x_1101));
+  assert (qas_nat h1 tmp == S.qmul (SI.qsquare_times (qas_nat h0 tmp) 6) (qas_nat h0 x_1101));
 
-  qsquare_times_in_place n tmp 4ul;
-  qmul_mont n tmp x_101 tmp; //tmp = r10
+  qsquare_times_in_place tmp 4ul;
+  qmul tmp tmp x_101; //tmp = r10
   let h2 = ST.get () in
-  assert (refls h2 tmp == S.qmul (SI.qsquare_times (refls h1 tmp) 4) (refls h0 x_101));
+  assert (qas_nat h2 tmp == S.qmul (SI.qsquare_times (qas_nat h1 tmp) 4) (qas_nat h0 x_101));
 
-  qsquare_times_in_place n tmp 3ul;
-  qmul_mont n tmp x_111 tmp; //tmp = r11
+  qsquare_times_in_place tmp 3ul;
+  qmul tmp tmp x_111; //tmp = r11
   let h3 = ST.get () in
-  assert (refls h3 tmp == S.qmul (SI.qsquare_times (refls h2 tmp) 3) (refls h0 x_111));
+  assert (qas_nat h3 tmp == S.qmul (SI.qsquare_times (qas_nat h2 tmp) 3) (qas_nat h0 x_111));
 
-  qsquare_times_in_place n tmp 5ul;
-  qmul_mont n tmp x_1001 tmp; //tmp = r12
+  qsquare_times_in_place tmp 5ul;
+  qmul tmp tmp x_1001; //tmp = r12
   let h4 = ST.get () in
-  assert (refls h4 tmp == S.qmul (SI.qsquare_times (refls h3 tmp) 5) (refls h0 x_1001));
+  assert (qas_nat h4 tmp == S.qmul (SI.qsquare_times (qas_nat h3 tmp) 5) (qas_nat h0 x_1001));
 
-  qsquare_times_in_place n tmp 6ul;
-  qmul_mont n tmp x_101 tmp; //tmp = r13
+  qsquare_times_in_place tmp 6ul;
+  qmul tmp tmp x_101; //tmp = r13
   let h5 = ST.get () in
-  assert (refls h5 tmp == S.qmul (SI.qsquare_times (refls h4 tmp) 6) (refls h0 x_101));
+  assert (qas_nat h5 tmp == S.qmul (SI.qsquare_times (qas_nat h4 tmp) 6) (qas_nat h0 x_101));
 
-  qsquare_times_in_place n tmp 10ul;
-  qmul_mont n tmp x_111 tmp; //tmp = r14
+  qsquare_times_in_place tmp 10ul;
+  qmul tmp tmp x_111; //tmp = r14
   let h6 = ST.get () in
-  assert (refls h6 tmp == S.qmul (SI.qsquare_times (refls h5 tmp) 10) (refls h0 x_111));
+  assert (qas_nat h6 tmp == S.qmul (SI.qsquare_times (qas_nat h5 tmp) 10) (qas_nat h0 x_111));
 
-  qsquare_times_in_place n tmp 4ul;
-  qmul_mont n tmp x_111 tmp; //tmp = r15
+  qsquare_times_in_place tmp 4ul;
+  qmul tmp tmp x_111; //tmp = r15
   let h7 = ST.get () in
-  assert (refls h7 tmp == S.qmul (SI.qsquare_times (refls h6 tmp) 4) (refls h0 x_111))
+  assert (qas_nat h7 tmp == S.qmul (SI.qsquare_times (qas_nat h6 tmp) 4) (qas_nat h0 x_111))
 
 
 // r16; ..;r23
 inline_for_extraction noextract
-val qinv6 (n tmp x8 x_11 x_1001 x_1011 x_1101: qelem) : Stack unit
+val qinv6 (tmp x8 x_11 x_1001 x_1011 x_1101: qelem) : Stack unit
   (requires fun h ->
-    live h n /\ live h tmp /\ live h x8 /\ live h x_11 /\
+    live h tmp /\ live h x8 /\ live h x_11 /\
     live h x_1001 /\ live h x_1011 /\ live h x_1101 /\
-    disjoint n tmp /\ disjoint n x8 /\ disjoint n x_11 /\
-    disjoint n x_1001 /\ disjoint n x_1011 /\ disjoint n x_1101 /\
     disjoint tmp x8 /\ disjoint tmp x_11 /\ disjoint tmp x_1001 /\
     disjoint tmp x_1011 /\ disjoint tmp x_1101 /\
-    linvs h tmp /\ linvs h x8 /\ linvs h x_11 /\ linvs h x_1001 /\
-    linvs h x_1011 /\ linvs h x_1101 /\ linv_ctxs h n)
+    qe_lt_q h tmp /\ qe_lt_q h x8 /\ qe_lt_q h x_11 /\
+    qe_lt_q h x_1001 /\ qe_lt_q h x_1011 /\ qe_lt_q h x_1101)
   (ensures  fun h0 _ h1 -> modifies (loc tmp) h0 h1 /\
-    linvs h1 tmp /\ refls h1 tmp == SI.qinv_r16_r23 (refls h0 tmp)
-      (refls h0 x8) (refls h0 x_11) (refls h0 x_1001) (refls h0 x_1011) (refls h0 x_1101))
+    qas_nat h1 tmp == SI.qinv_r16_r23 (qas_nat h0 tmp)
+      (qas_nat h0 x8) (qas_nat h0 x_11) (qas_nat h0 x_1001) (qas_nat h0 x_1011) (qas_nat h0 x_1101) /\
+    qe_lt_q h1 tmp)
 
-let qinv6 n tmp x8 x_11 x_1001 x_1011 x_1101 =
+let qinv6 tmp x8 x_11 x_1001 x_1011 x_1101 =
   let h0 = ST.get () in
-  qsquare_times_in_place n tmp 9ul;
-  qmul_mont n tmp x8 tmp; //tmp = r16
+  qsquare_times_in_place tmp 9ul;
+  qmul tmp tmp x8; //tmp = r16
   let h1 = ST.get () in
-  assert (refls h1 tmp == S.qmul (SI.qsquare_times (refls h0 tmp) 9) (refls h0 x8));
+  assert (qas_nat h1 tmp == S.qmul (SI.qsquare_times (qas_nat h0 tmp) 9) (qas_nat h0 x8));
 
-  qsquare_times_in_place n tmp 5ul;
-  qmul_mont n tmp x_1001 tmp; //tmp = r17
+  qsquare_times_in_place tmp 5ul;
+  qmul tmp tmp x_1001; //tmp = r17
   let h2 = ST.get () in
-  assert (refls h2 tmp == S.qmul (SI.qsquare_times (refls h1 tmp) 5) (refls h0 x_1001));
+  assert (qas_nat h2 tmp == S.qmul (SI.qsquare_times (qas_nat h1 tmp) 5) (qas_nat h0 x_1001));
 
-  qsquare_times_in_place n tmp 6ul;
-  qmul_mont n tmp x_1011 tmp; //tmp = r18
+  qsquare_times_in_place tmp 6ul;
+  qmul tmp tmp x_1011; //tmp = r18
   let h3 = ST.get () in
-  assert (refls h3 tmp == S.qmul (SI.qsquare_times (refls h2 tmp) 6) (refls h0 x_1011));
+  assert (qas_nat h3 tmp == S.qmul (SI.qsquare_times (qas_nat h2 tmp) 6) (qas_nat h0 x_1011));
 
-  qsquare_times_in_place n tmp 4ul;
-  qmul_mont n tmp x_1101 tmp; //tmp = r19
+  qsquare_times_in_place tmp 4ul;
+  qmul tmp tmp x_1101; //tmp = r19
   let h4 = ST.get () in
-  assert (refls h4 tmp == S.qmul (SI.qsquare_times (refls h3 tmp) 4) (refls h0 x_1101));
+  assert (qas_nat h4 tmp == S.qmul (SI.qsquare_times (qas_nat h3 tmp) 4) (qas_nat h0 x_1101));
 
-  qsquare_times_in_place n tmp 5ul;
-  qmul_mont n tmp x_11 tmp; //tmp = r20
+  qsquare_times_in_place tmp 5ul;
+  qmul tmp tmp x_11; //tmp = r20
   let h5 = ST.get () in
-  assert (refls h5 tmp == S.qmul (SI.qsquare_times (refls h4 tmp) 5) (refls h0 x_11));
+  assert (qas_nat h5 tmp == S.qmul (SI.qsquare_times (qas_nat h4 tmp) 5) (qas_nat h0 x_11));
 
-  qsquare_times_in_place n tmp 6ul;
-  qmul_mont n tmp x_1101 tmp; //tmp = r21
+  qsquare_times_in_place tmp 6ul;
+  qmul tmp tmp x_1101; //tmp = r21
   let h6 = ST.get () in
-  assert (refls h6 tmp == S.qmul (SI.qsquare_times (refls h5 tmp) 6) (refls h0 x_1101));
+  assert (qas_nat h6 tmp == S.qmul (SI.qsquare_times (qas_nat h5 tmp) 6) (qas_nat h0 x_1101));
 
-  qsquare_times_in_place n tmp 10ul;
-  qmul_mont n tmp x_1101 tmp; //tmp = r22
+  qsquare_times_in_place tmp 10ul;
+  qmul tmp tmp x_1101; //tmp = r22
   let h7 = ST.get () in
-  assert (refls h7 tmp == S.qmul (SI.qsquare_times (refls h6 tmp) 10) (refls h0 x_1101));
+  assert (qas_nat h7 tmp == S.qmul (SI.qsquare_times (qas_nat h6 tmp) 10) (qas_nat h0 x_1101));
 
-  qsquare_times_in_place n tmp 4ul;
-  qmul_mont n tmp x_1001 tmp; //tmp = r23
+  qsquare_times_in_place tmp 4ul;
+  qmul tmp tmp x_1001; //tmp = r23
   let h8 = ST.get () in
-  assert (refls h8 tmp == S.qmul (SI.qsquare_times (refls h7 tmp) 4) (refls h0 x_1001))
+  assert (qas_nat h8 tmp == S.qmul (SI.qsquare_times (qas_nat h7 tmp) 4) (qas_nat h0 x_1001))
 
 
 //r24; r25
 inline_for_extraction noextract
-val qinv7 (n tmp f x6: qelem) : Stack unit
+val qinv7 (tmp f x6: qelem) : Stack unit
   (requires fun h ->
-    live h n /\ live h tmp /\ live h f /\ live h x6 /\
-    disjoint n tmp /\ disjoint n f /\ disjoint n x6 /\
+    live h tmp /\ live h f /\ live h x6 /\
     disjoint tmp f /\ disjoint tmp x6 /\
-    linvs h tmp /\ linvs h f /\ linvs h x6 /\ linv_ctxs h n)
+    qe_lt_q h tmp /\ qe_lt_q h f /\ qe_lt_q h x6)
   (ensures  fun h0 _ h1 -> modifies (loc tmp) h0 h1 /\
-    linvs h1 tmp /\ refls h1 tmp == SI.qinv_r24_r25 (refls h0 tmp) (refls h0 f) (refls h0 x6))
+    qas_nat h1 tmp == SI.qinv_r24_r25 (qas_nat h0 tmp) (qas_nat h0 f) (qas_nat h0 x6) /\
+    qe_lt_q h1 tmp)
 
-let qinv7 n tmp f x6 =
+let qinv7 tmp f x6 =
   let h0 = ST.get () in
-  qsquare_times_in_place n tmp 6ul;
-  qmul_mont n tmp f tmp; //tmp = r23
+  qsquare_times_in_place tmp 6ul;
+  qmul tmp tmp f; //tmp = r23
   let h1 = ST.get () in
-  assert (refls h1 tmp == S.qmul (SI.qsquare_times (refls h0 tmp) 6) (refls h0 f));
+  assert (qas_nat h1 tmp == S.qmul (SI.qsquare_times (qas_nat h0 tmp) 6) (qas_nat h0 f));
 
-  qsquare_times_in_place n tmp 8ul;
-  qmul_mont n tmp x6 tmp; //tmp = r24
+  qsquare_times_in_place tmp 8ul;
+  qmul tmp tmp x6; //tmp = r24
   let h2 = ST.get () in
-  assert (refls h2 tmp == S.qmul (SI.qsquare_times (refls h1 tmp) 8) (refls h0 x6))
+  assert (qas_nat h2 tmp == S.qmul (SI.qsquare_times (qas_nat h1 tmp) 8) (qas_nat h0 x6))
 
 
 inline_for_extraction noextract
-val qinv8 (n tmp f x_11 x_101 x_111 x_1001 x_1011 x_1101: qelem) : Stack unit
+val qinv8 (tmp f x_11 x_101 x_111 x_1001 x_1011 x_1101: qelem) : Stack unit
   (requires fun h ->
-    live h n /\ live h tmp /\ live h f /\ live h x_11 /\
+    live h tmp /\ live h f /\ live h x_11 /\
     live h x_101 /\ live h x_111 /\ live h x_1001 /\
     live h x_1011 /\ live h x_1101 /\
-    disjoint n tmp /\ disjoint n f /\ disjoint n x_11 /\
-    disjoint n x_101 /\ disjoint n x_111 /\ disjoint n x_1001 /\
-    disjoint n x_1011 /\ disjoint n x_1101 /\ disjoint tmp f /\
-    disjoint tmp x_11 /\ disjoint tmp x_101 /\ disjoint tmp x_111 /\
-    disjoint tmp x_1001 /\ disjoint tmp x_1011 /\ disjoint tmp x_1101 /\
-    linvs h f /\ linvs h x_11 /\ linvs h x_101 /\ linvs h x_111 /\
-    linvs h x_1001 /\ linvs h x_1011 /\ linvs h x_1101 /\ linv_ctxs h n)
+    disjoint tmp f /\ disjoint tmp x_11 /\ disjoint tmp x_101 /\
+    disjoint tmp x_111 /\ disjoint tmp x_1001 /\ disjoint tmp x_1011 /\
+    disjoint tmp x_1101 /\
+    qe_lt_q h f /\ qe_lt_q h x_11 /\ qe_lt_q h x_101 /\
+    qe_lt_q h x_111 /\ qe_lt_q h x_1001 /\ qe_lt_q h x_1011 /\
+    qe_lt_q h x_1101)
   (ensures  fun h0 _ h1 -> modifies (loc tmp) h0 h1 /\
-    linvs h1 tmp /\ refls h1 tmp == SI.qinv_r0_r25 (refls h0 f)
-      (refls h0 x_11) (refls h0 x_101) (refls h0 x_111)
-      (refls h0 x_1001) (refls h0 x_1011) (refls h0 x_1101))
+    qas_nat h1 tmp == SI.qinv_r0_r25 (qas_nat h0 f)
+      (qas_nat h0 x_11) (qas_nat h0 x_101) (qas_nat h0 x_111)
+      (qas_nat h0 x_1001) (qas_nat h0 x_1011) (qas_nat h0 x_1101) /\
+    qe_lt_q h1 tmp)
 
-let qinv8 n tmp f x_11 x_101 x_111 x_1001 x_1011 x_1101 =
+let qinv8 tmp f x_11 x_101 x_111 x_1001 x_1011 x_1101 =
   push_frame ();
   let x6 = create_qelem () in
   let x8 = create_qelem () in
   let x14 = create_qelem () in
 
   let h1 = ST.get () in
-  qinv2 n x_11 x_1011 x_1101 x6 x8 x14; //x6; x8; x14
+  qinv2 x_11 x_1011 x_1101 x6 x8 x14; //x6; x8; x14
   let h2 = ST.get () in
   assert (modifies (loc x6 |+| loc x8 |+| loc x14) h1 h2);
 
-  qinv3 n tmp x14; //x28; x56; r0; r1
+  qinv3 tmp x14; //x28; x56; r0; r1
   let h3 = ST.get () in
   assert (modifies (loc tmp) h2 h3);
 
-  qinv4 n tmp x_101 x_111 x_1011; //r2; ..; r8
+  qinv4 tmp x_101 x_111 x_1011; //r2; ..; r8
   let h4 = ST.get () in
   assert (modifies (loc tmp) h3 h4);
 
-  qinv5 n tmp x_101 x_111 x_1001 x_1101; //r9; ..; r15
+  qinv5 tmp x_101 x_111 x_1001 x_1101; //r9; ..; r15
   let h5 = ST.get () in
   assert (modifies (loc tmp) h4 h5);
 
-  qinv6 n tmp x8 x_11 x_1001 x_1011 x_1101; //r16; ..; r23
+  qinv6 tmp x8 x_11 x_1001 x_1011 x_1101; //r16; ..; r23
   let h6 = ST.get () in
   assert (modifies (loc tmp) h5 h6);
 
-  qinv7 n tmp f x6; //r24; r25
+  qinv7 tmp f x6; //r24; r25
   let h7 = ST.get () in
   assert (modifies (loc tmp) h6 h7);
   pop_frame ()
 
 
 inline_for_extraction noextract
-val qinv_ (n out f: qelem) : Stack unit
+val qinv_ (out f: qelem) : Stack unit
   (requires fun h ->
-    live h n /\ live h out /\ live h f /\
-    disjoint n out /\ disjoint n f /\ disjoint out f /\
-    linvs h f /\ linv_ctxs h n)
+    live h out /\ live h f /\ disjoint out f /\
+    qe_lt_q h f)
   (ensures  fun h0 _ h1 -> modifies (loc out) h0 h1 /\
-    linvs h1 out /\ refls h1 out == SI.qinv (refls h0 f))
+    qas_nat h1 out == SI.qinv (qas_nat h0 f)  /\
+    qe_lt_q h1 out)
 
 #set-options "--z3rlimit 150"
 
-let qinv_ n out f =
+let qinv_ out f =
   push_frame ();
   let x_10 = create_qelem () in
   let x_11 = create_qelem () in
@@ -553,8 +474,8 @@ let qinv_ n out f =
   let x_1011 = create_qelem () in
   let x_1101 = create_qelem () in
 
-  qinv1 n f x_10 x_11 x_101 x_111 x_1001 x_1011 x_1101;
-  qinv8 n out f x_11 x_101 x_111 x_1001 x_1011 x_1101;
+  qinv1 f x_10 x_11 x_101 x_111 x_1001 x_1011 x_1101;
+  qinv8 out f x_11 x_101 x_111 x_1001 x_1011 x_1101;
   pop_frame ()
 
 
@@ -568,14 +489,6 @@ val qinv (out f: qelem) : Stack unit
 
 [@CInline]
 let qinv out f =
-  push_frame ();
-  let fM = create_qelem () in
-  let outM = create_qelem () in
-  let n = create_qelem () in
-  make_u64_4 n (make_order_k256 ());
-  to_mont n f fM;
   let h0 = ST.get () in
-  SI.qinv_is_qinv_lemma (refls h0 fM);
-  qinv_ n outM fM;
-  from_mont n outM out;
-  pop_frame ()
+  SI.qinv_is_qinv_lemma (qas_nat h0 f);
+  qinv_ out f
